Volume1/Auto.v
@@ -221,7 +221,7 @@ Hint Unfold is_fortytwo : core.
 Example auto_example_7' : forall x,
   (x <= 42 /\ 42 <= x) -> is_fortytwo x.
 Proof.
-  auto. (* try also: info_auto. *)
+  info_auto. (* try also: info_auto. *)
 Qed.
 
 (** Let's take a first pass over [ceval_deterministic] to simplify the
